towards correctness

src/Util/FisherYates/Correctness.dfy
@@ -17,6 +17,10 @@ module FisherYates.Correctness {
    Definitions
   ************/
 
+  predicate IsPermutationOf<T(==)>(p: seq<T>, s: seq<T>) {
+    && multiset(p) == multiset(s)
+    && |p| == |s|
+  }
 
   // Calculates the number n of permutations of a sequence s
   function NumberOfPermutationsOf<T(==)>(s: seq<T>): (n: nat)
@@ -29,57 +33,103 @@ module FisherYates.Correctness {
       var length := |s|;
       (length / multiplicity) * NumberOfPermutationsOf(s[1..])
   }  
-  /*
-  Proof of correctness sketch:
-  Let set(s) = { x_0, ..., x_n } and |x_k| == multiplicity of x_k in s. W.l.o.g. assume s[0] == x_0, then:
-
-    |Perm(s)| 
-  == // Well-known formula
-    |s|! / (|x_0|! * ... * |x_n|!) 
-  == 
-    |s| * (|s|-1)! 
-    / 
-    |x_0| * (|x_0|-1)! * ... * |x_n|!   // if |x_0| >= 1, otherwise |x_0| * |x_1|! * ... * |x_n|! 
-  == 
-    |s| / |x_0|
-    * 
-    (|s|-1)! / (|x_0|-1)! * ... * |x_n|!  // if |x_0| >= 1, otherwise (|s|-1)!  * |x_1|! * ... * |x_n|! 
-  ==
-    length / multiplicity
-    *
-    |Perm(s[1..])| // since |s[1..]| == |s| - 1 and multiplicity of x_0 in s[1..] is one less than in s, and the multiplicity of x_k != x_0 in s[1..] is the same as in s
-  */
-
-  function NumberOfPermutationsOfAlternative<T(==)>(s: seq<T>, i: nat := 0): (n: nat)
-    requires i <= |s|
-    decreases |s| - i
-  {
-    if |s| <= 1 || i == |s| then
-      1
-    else
-      var multiplicity := multiset(s[i..])[s[i]];
-      var length := |s[i..]|;
-      (length / multiplicity) * NumberOfPermutationsOfAlternative(s, i+1)
-  }
 
   /*******
    Lemmas
   *******/
 
-  lemma NumberOfPermutationsEquivalence<T(==)>(s: seq<T>, i: nat)
-    requires i <= |s|
-    ensures NumberOfPermutationsOfAlternative(s, i) == NumberOfPermutationsOf(s[i..])
-    decreases |s| - i
+  lemma CorrectnessFisherYates<T(!new)>(xs: seq<T>, p: seq<T>)
+    requires IsPermutationOf(p, xs)
+    ensures
+      var e := iset s | Model.Shuffle(xs)(s).Equals(p);
+      && e in Rand.eventSpace
+      && Rand.prob(e) == 1.0 / (NumberOfPermutationsOf(xs) as real)
   {
-    if |s| <= 1 || i == |s| {
+    var e := iset s | Model.Shuffle(xs)(s).Equals(p);
+    var e' := iset s | Model.Shuffle(xs, 0)(s).Result? && Model.Shuffle(xs, 0)(s).value[0..] == p[0..];
+    assert e == e';
+    CorrectnessFisherYatesGeneral(xs, p, 0);
+  }
+
+  lemma CorrectnessFisherYatesGeneral<T(!new)>(xs: seq<T>, p: seq<T>, i: nat)
+    requires i <= |xs|
+    requires i <= |p| 
+    requires IsPermutationOf(p[i..], xs[i..])
+    decreases |xs| - i
+    ensures
+      var e := iset s | Model.Shuffle(xs, i)(s).Result? && Model.Shuffle(xs, i)(s).value[i..] == p[i..];
+      && e in Rand.eventSpace
+      && Rand.prob(e) == 1.0 / (NumberOfPermutationsOf(xs[i..]) as real)
+  {
+    var e := iset s | Model.Shuffle(xs, i)(s).Result? && Model.Shuffle(xs, i)(s).value[i..] == p[i..];
+    if |xs[i..]| <= 1 {
+      assert e == Measures.SampleSpace() by {
+        forall s 
+          ensures s in e
+        {
+          calc {
+            s in e;
+            Model.Shuffle(xs, i)(s).Result? && Model.Shuffle(xs, i)(s).value[i..] == p[i..];
+            { assert Model.Shuffle(xs, i)(s) == Monad.Return(xs)(s); }
+            Monad.Return(xs)(s).Result? && Monad.Return(xs)(s).value[i..] == p[i..];
+            { assert Monad.Return(xs)(s).value == xs; }
+            xs[i..] == p[i..];
+            if |xs[i..]| == 0 then [] == p[i..] else [xs[i]] == p[i..];
+            { assert |xs[i..]| == |p[i..]|; }
+            if |xs[i..]| == 0 then true else [xs[i]] == [p[i]];
+            { assert multiset(p[i..]) == multiset(xs[i..]); }
+            true;
+          }
+        }
+      }
+      Rand.ProbIsProbabilityMeasure();
+      assert Measures.IsProbability(Rand.eventSpace, Rand.prob);
     } else {
-      NumberOfPermutationsEquivalence(s, i+1);
+      var h := Uniform.Model.IntervalSample(i, |xs|);
+      assert HIsIndependent: Independence.IsIndep(h) by {
+        Uniform.Correctness.IntervalSampleIsIndep(i, |xs|);
+      }
+      var multiplicity := multiset(xs[i..])[xs[i]];
+      var length := |xs[i..]|;
+      var A := iset j | i <= j < |xs| && xs[j] == p[i];
+      assert A != iset{} by {
+        assume {:axiom} false;
+        assert IsPermutationOf(p[i..], xs[i..]);
+      }
+      var j :| j in A;
+      var ys := Model.Swap(xs, i, j);
+      var e' := iset s | Model.Shuffle(ys, i+1)(s).Result? && Model.Shuffle(ys, i+1)(s).value[i+1..] == p[i+1..];
+            assume {:axiom} false;
+        /*
+      assert DecomposeE: e == (iset s | s in Monad.BitstreamsWithValueIn(h, A) && s in Monad.BitstreamsWithRestIn(h, e')) by {
+        assume {:axiom} false;
+      } 
+             calc {
+        Rand.prob(e);
+        Rand.prob(iset s | Model.Shuffle(xs, i)(s).Result? && Model.Shuffle(xs, i)(s).value[i..] == p[i..]);
+        { reveal DecomposeE; }
+        Rand.prob(iset s | s in Monad.BitstreamsWithValueIn(h, A) && s in Monad.BitstreamsWithRestIn(h, e'));
+        { reveal HIsIndependent; Independence.ResultsIndependent(h, A, e'); }
+        Rand.prob(iset s | s in Monad.BitstreamsWithValueIn(h, A)) * Rand.prob(e');
+        { assume {:axiom} false; }
+        //{ CorrectnessMultiset(xs, p[i], i); CorrectnessFisherYatesGeneral(xs, p, i+1); }
+        (multiplicity as real / length as real) * (1.0 / (NumberOfPermutationsOf(xs[i+1..]) as real));
+        { assume {:axiom} false; }
+        (1.0 / ((length as real) / (multiplicity as real))) *  (1.0 / (NumberOfPermutationsOf(xs[i+1..]) as real));
+        { assume {:axiom} false; }
+        (1.0 / ((length / multiplicity) as real)) *  (1.0 / (NumberOfPermutationsOf(xs[i+1..]) as real));
+        { assume {:axiom} false; assert 1.0 * 1.0 == 1.0; assert ((length / multiplicity) as real) * (NumberOfPermutationsOf(xs[i+1..]) as real) == (((length / multiplicity) * NumberOfPermutationsOf(xs[i+1..])) as real); }
+        1.0 / (((length / multiplicity) * NumberOfPermutationsOf(xs[i+1..])) as real);    
+        { assume {:axiom} false; assert xs[i+1..] == xs[i..][1..]; }        
+        1.0 / (((length / multiplicity) * NumberOfPermutationsOf(xs[i..][1..])) as real);  
+        { assume {:axiom} false; }      
+        1.0 / (NumberOfPermutationsOf(xs[i..]) as real);
+      } */
     }
   }
 
   lemma CorrectnessMultiset<T>(xs: seq<T>, x: T, i: nat := 0)
     requires i <= |xs| - 1
-    requires x in xs[i..]
     decreases |xs| - i
     ensures 
       var A := iset j: int | i <= j < |xs| && xs[j] == x;
@@ -94,21 +144,32 @@ module FisherYates.Correctness {
     var multiplicity := multiset(xs[i..])[x];
     var length := |xs[i..]|;
     if i == |xs| - 1 {
-      assert A == iset{ |xs| - 1 };
-      assert e == Uniform.Correctness.SampleEquals(1, 0);
-      Uniform.Correctness.UniformFullCorrectness(1, 0);    
-      assert multiplicity == 1;
       assert length == 1;
+      if xs[i] == x {
+        assert A == iset{ |xs| - 1 };
+        assert multiplicity == 1;
+        Uniform.Correctness.UniformFullIntervalCorrectness(i, |xs|, i);
+      } else {
+        assert A == iset{};
+        assert e == iset{};
+        assert multiplicity == 0;
+        Rand.ProbIsProbabilityMeasure();
+        assert Measures.IsPositive(Rand.eventSpace, Rand.prob);
+      }
     } else {
       var A' := iset j: int | i+1 <= j < |xs| && xs[j] == x;
       var e' := Monad.BitstreamsWithValueIn(Uniform.Model.IntervalSample(i+1, |xs|), A');
+      assert e'Equality: e' == Monad.BitstreamsWithValueIn(Uniform.Model.IntervalSample(i, |xs|), A') by {
+        assume {:axiom} false;
+      }
+      var e'':= (iset s | Uniform.Model.IntervalSample(i, |xs|)(s).Equals(i as int));
       var multiplicity' := multiset(xs[i+1..])[x];
       var length' := |xs[i+1..]|;
       assert InductionHypothesis: e' in Rand.eventSpace && Rand.prob(e') == (multiplicity' as real) / (length' as real) by {
         CorrectnessMultiset(xs, x, i+1);
       }
       assert length == 1 + length';
-      if x == xs[i] {
+      if xs[i] == x {
         assert multiplicity == 1 + multiplicity' by {
           calc {
             multiplicity;
@@ -128,10 +189,10 @@ module FisherYates.Correctness {
           Monad.BitstreamsWithValueIn(Uniform.Model.IntervalSample(i, |xs|), A' + iset{i as int});
           { Monad.BitstreamsWithValueInJoin(Uniform.Model.IntervalSample(i, |xs|), A', iset{i as int}); }
           Monad.BitstreamsWithValueIn(Uniform.Model.IntervalSample(i, |xs|), A') + Monad.BitstreamsWithValueIn(Uniform.Model.IntervalSample(i, |xs|), iset{i as int});
+          { assume {:axiom} false; }
           Monad.BitstreamsWithValueIn(Uniform.Model.IntervalSample(i+1, |xs|), A') + (iset s | Uniform.Model.IntervalSample(i, |xs|)(s).Equals(i as int));
-          e' + (iset s | Uniform.Model.IntervalSample(i, |xs|)(s).Equals(i as int));
+          e' + e'';
         }
-        var e'':= (iset s | Uniform.Model.IntervalSample(i, |xs|)(s).Equals(i as int));
         assert e''inEventSpace: e'' in Rand.eventSpace by {
           Uniform.Correctness.UniformFullIntervalCorrectness(i, |xs|, i);
         }
@@ -173,12 +234,15 @@ module FisherYates.Correctness {
           Monad.BitstreamsWithValueIn(Uniform.Model.IntervalSample(i, |xs|), A);
           { assert A == A'; }
           Monad.BitstreamsWithValueIn(Uniform.Model.IntervalSample(i, |xs|), A');
-          Monad.BitstreamsWithValueIn(Uniform.Model.IntervalSample(i+1, |xs|), A');
+          { reveal e'Equality; }
           e';
         }
         calc {
           Rand.prob(e);
           Rand.prob(e');
+          { reveal InductionHypothesis; }
+          (multiplicity' as real) / (length' as real);
+          { assume {:axiom} false; }
           (multiplicity' as real) / ((1 + length') as real);
           (multiplicity as real) / (length as real);
         }
@@ -186,58 +250,6 @@ module FisherYates.Correctness {
     }
   }
 
-  lemma CorrectnessFisherYates<T(!new)>(xs: seq<T>, p: seq<T>)
-    requires multiset(p) == multiset(xs)
-    requires |p| == |xs|
-    ensures
-      var e := iset s | Model.Shuffle(xs)(s).Equals(p);
-      && e in Rand.eventSpace
-      && Rand.prob(e) == 1.0 / (NumberOfPermutationsOf(xs) as real)
-  {
-    CorrectnessFisherYatesGeneral(xs, p, 0);
-  }
 
-  lemma CorrectnessFisherYatesGeneral<T(!new)>(xs: seq<T>, p: seq<T>, i: nat)
-    requires i <= |xs|
-    requires multiset(p) == multiset(xs)
-    requires |p| == |xs|
-    decreases |xs| - i
-    ensures
-      var e := iset s | Model.Shuffle(xs, i)(s).Map(ys => ys[i..]).Equals(p[i..]);
-      && e in Rand.eventSpace
-      && Rand.prob(e) == 1.0 / (NumberOfPermutationsOfAlternative(xs, i) as real)
-  {
-    var e := iset s | Model.Shuffle(xs, i)(s).Map(ys => ys[i..]).Equals(p[i..]);
-    if |xs| == 0 {
-      assert e == iset s | true;
-      assert NumberOfPermutationsOfAlternative(xs, i) == 1;
-    } else {
-      assume {:axiom} false;
-      var h := Uniform.Model.IntervalSample(i, |xs|);
-      assert Independence.IsIndep(h) by {
-        Uniform.Correctness.IntervalSampleIsIndep(i, |xs|);
-      }
-      var multiplicity := multiset(xs[i..])[p[i]];
-      var length := |xs[i..]|;
-      var A := iset j | i <= j < |xs| && xs[j] == p[i];
-      var j :| j in A;
-      var ys := Model.Swap(xs, i, j);
-      var E := iset s | Model.Shuffle(ys, i+1)(s).Map(ys => ys[i+1..]).Equals(p[i+1..]);
-
-      calc {
-        Rand.prob(e);
-        Rand.prob(iset s | Model.Shuffle(xs, i)(s).Map(ys => ys[i..]).Equals(p[i..]));
-        Rand.prob(iset s | s in Monad.BitstreamsWithValueIn(h, A) && s in Monad.BitstreamsWithRestIn(h, E));
-        Rand.prob(iset s | s in Monad.BitstreamsWithValueIn(h, A)) * Rand.prob(E);
-        { CorrectnessMultiset(xs, p[i], i); CorrectnessFisherYatesGeneral(ys, p, i+1); }
-        (multiplicity as real / length as real) * (1.0 / (NumberOfPermutationsOfAlternative(xs, i+1) as real));
-        (1.0 / ((length as real) / (multiplicity as real))) *  (1.0 / (NumberOfPermutationsOfAlternative(xs, i+1) as real));
-        (1.0 / ((length / multiplicity) as real)) *  (1.0 / (NumberOfPermutationsOfAlternative(xs, i+1) as real));
-        { assert 1.0 * 1.0 == 1.0; assert ((length / multiplicity) as real) * (NumberOfPermutationsOfAlternative(xs, i+1) as real) == ((length / multiplicity) * NumberOfPermutationsOfAlternative(xs, i+1)) as real; }
-        1.0 / ((length / multiplicity) * NumberOfPermutationsOfAlternative(xs, i+1)) as real;
-        1.0 / (NumberOfPermutationsOfAlternative(xs, i) as real);
-      }
-    }
-  }
 
 }
