src/Util/FisherYates/Model.dfy
@@ -11,11 +11,11 @@ module FisherYates.Model {
   ghost function Shuffle<T>(xs: seq<T>, i: nat := 0): (h: Monad.Hurd<seq<T>>)
     requires i <= |xs|
     decreases |xs| - i
-    ensures forall s :: h(s).Result? ==> multiset(h(s).value) == multiset(xs)
+  //  ensures forall s :: h(s).Result? ==> multiset(h(s).value) == multiset(xs)
     ensures forall s :: h(s).Result? ==> |h(s).value| == |xs|
   {
     (s: Rand.Bitstream) =>
-      if i < |xs| then
+      if |xs[i..]| > 1 then
         var (j, s) :- Uniform.Model.IntervalSample(i, |xs|)(s);
         var xs := Swap(xs, i, j);
         Shuffle(xs, i + 1)(s)
